Update L_Star.lean

L_Star.lean
@@ -3,14 +3,51 @@ structure DFAState := (name : String) deriving BEq
 structure FiniteAutomaton (Alph : List Char) :=
 (Q : List DFAState)
 (S : DFAState)
+(start_in_Q : S ∈ Q)
 (δ : DFAState → Char → DFAState)
+(trans_in_Q : ∀q ∈ Q, ∀a ∈ Alph, δ q a ∈ Q)
 (Accept : List DFAState)
+(accept_in_Q : a ∈ Accept → a ∈ Q)
 
 def validateWord (DFA : FiniteAutomaton Alph)
   (word : List Char) (curState : DFAState) : Bool :=
   match word with
   | [] => DFA.Accept.contains curState
   | w :: lst => validateWord DFA lst (DFA.δ curState w)
+
+def minimal_regularity (Alph : List Char) (Mem : String → Bool) : Prop :=
+  ∃automaton : FiniteAutomaton Alph, (∀w : List Char, Mem (w.toString) = validateWord automaton w automaton.S
+  ∧ ∀automaton2 : FiniteAutomaton Alph, ∀w : List Char, (Mem (w.toString) = validateWord automaton2 w automaton2.S
+  → sizeOf automaton2.Q >= sizeOf automaton.Q))
+
+def findAcceptingStates (Q : List String) (Mem : String → Bool) : List String :=
+  match Q with
+  | w :: rem => if Mem w then w :: findAcceptingStates rem Mem else findAcceptingStates rem Mem
+  | [] => []
+
+theorem accepting_in_q : a ∈ findAcceptingStates Q Mem → a ∈ Q := by
+  induction Q with
+  | nil => {
+    intro h
+    assumption
+  }
+  | cons b tail tail_ih => {
+    intro h
+    simp [findAcceptingStates] at h
+    split at h
+    case cons.isTrue => rw [List.mem_cons] at h
+                        rw [List.mem_cons]
+                        apply Or.elim h
+                        case left => apply Or.intro_left
+                        case right => intro h2
+                                      have h3 : a ∈ tail := tail_ih h2
+                                      apply Or.intro_right
+                                      exact h3
+    case cons.isFalse => have h2 : a ∈ tail := tail_ih h
+                         rw [List.mem_cons]
+                         apply Or.intro_right
+                         exact h2
+  }
 
 def T_Equivalent (Alph : List Char) (T : List String)
   (w1 : String) (w2 : String) (Mem : String → Bool)
@@ -35,6 +72,30 @@ def for_Alph (Alph : List Char) (Alph_loop : List Char)
                     | none => for_Alph Alph rem Q T q Mem
   | [] => none
 
+def toAutomaton (Alph : List Char) (T : List String) (Q : List String) (Mem : String → Bool)
+  (h : "" ∈ Q): FiniteAutomaton Alph :=
+  {Q := Q.map (fun x => {name := x}), S := {name := ""},
+    Accept := (findAcceptingStates Q Mem).map (fun x => {name := x}), δ := fun q0 => fun a =>
+    match for_Q2 Alph Q Q T q0.name a Mem with
+    | some (s, c) => {name := s ++ Char.toString c}
+    | none => {name := ""},
+    start_in_Q := by
+      rw [List.mem_map]
+      exact ⟨"", by apply And.intro
+                    case right => rfl
+                    case left => exact h⟩
+    ,
+    accept_in_Q := by
+      intro a
+      intro hy
+      rw [List.mem_map]
+      rw [List.mem_map] at hy
+      match hy with
+      | ⟨w, hw⟩ => exact ⟨w, by apply And.intro
+                                case right => exact hw.right
+                                case left => exact accepting_in_q hw.left⟩
+  }
+
 def complete_loop (Alph : List Char) (Q : List String) (Q_Iterator : List String)
   (T : List String) (Mem : String → Bool)
   : Option (String × Char) :=
@@ -44,30 +105,16 @@ def complete_loop (Alph : List Char) (Q : List String) (Q_Iterator : List String
                      | none => complete_loop Alph Q rem T Mem
   | [] => none
 
-def complete (Alph : List Char) (T : List String) (Q : List String)
-  (Q_New : List String) (Mem : String → Bool)
-  : List String :=
+def complete (Alph : List Char) (T : List String) (Q : List String) (Mem : String → Bool)
+  (reg : minimal_regularity Alph Mem): List String :=
   match complete_loop Alph Q Q T Mem with
-  | some (s, c) => complete Alph T Q ((s ++ Char.toString c) :: Q_New) Mem
-  | none => Q_New
+  | some (s, c) => complete Alph T ((s ++ Char.toString c) :: Q) Mem reg
+  | none => Q
 
-def findAcceptingStates (Q : List String) (Mem : String → Bool) : List String :=
-  match Q with
-  | w :: rem => if Mem w then w :: findAcceptingStates rem Mem else findAcceptingStates rem Mem
+def getSuffixes (w : List Char) : List String :=
+  match w with
+  | _ :: tail => tail.toString :: getSuffixes tail
   | [] => []
-
-def toAutomaton (Alph : List Char) (T : List String) (Q : List String) (Mem : String → Bool)
-  : FiniteAutomaton Alph :=
-  {Q := Q.map (fun x => {name := x}), S := {name := ""},
-    Accept := (findAcceptingStates Q Mem).map (fun x => {name := x}), δ := fun q0 => fun a =>
-    match for_Q2 Alph Q Q T q0.name a Mem with
-    | some (s, c) => {name := s ++ Char.toString c}
-    | none => {name := ""}
-  }
-
-def getSuffixes (w : String) : List String :=
-  tail :: getSuffixes tail
-  where tail := w.drop 1
 
 def removeStringDuplicates (l : List String) : List String :=
   match l with
@@ -78,7 +125,8 @@ def removeStringDuplicates (l : List String) : List String :=
 
 def LStar (Alph : List Char) (Q : List String) (T : List String) (Mem : String → Bool)
   (Eqiv : FiniteAutomaton Alph → Option (String))
+  (reg : minimal_regularity Alph Mem)
   : FiniteAutomaton Alph := match Eqiv dfa with
     | none => dfa
-    | some w => LStar Alph Q_compl (removeStringDuplicates (T ++ getSuffixes w).mergeSort) Mem Eqiv
-    where Q_compl := complete Alph T Q Q Mem; dfa := toAutomaton Alph T Q_compl Mem
+    | some w => LStar Alph Q_compl (removeStringDuplicates (T ++ getSuffixes w.data).mergeSort) Mem Eqiv reg
+    where Q_compl := complete Alph T Q Mem reg; dfa := toAutomaton Alph T Q_compl Mem 
